updates

src/Framework/CompKnown.v
@@ -31,13 +31,15 @@ Module M.
 
   Section Comp_n.
 
-    Definition Top_n n m := Cross (Cross (C0.Top_n n) (fun e1 e2 => AM.trans_correct_top (AM.analyze e1) e1 e2)) (C1.Top_n m).
+    Variable K : known_map.
 
-    Definition V_n n m := Cross (Cross (C0.V_n n) (fun v1 v2 => exists K, forall k, AM.V K k v1 v2)) (C1.V_n m).
+    Definition Top_n n m := Cross (Cross (C0.Top_n n) (fun e1 e2 => AM.trans_correct_top K e1 e2)) (C1.Top_n m).
 
-    Definition R_n n m := Cross (Cross (C0.R_n n) (fun v1 v2 => exists K, forall k, AM.R K k v1 v2)) (C1.R_n m).
+    Definition V_n n m := Cross (Cross (C0.V_n n) (fun v1 v2 => forall k, AM.V K k v1 v2)) (C1.V_n m).
 
-    Definition G_n n m Γ1 Γ2 := Cross (Cross (C0.G_n n Γ1 Γ2) (fun ρ1 ρ2 => forall K k, AM.G_top K k Γ1 ρ1 Γ2 ρ2)) (C1.G_n m Γ1 Γ2).
+    Definition R_n n m := Cross (Cross (C0.R_n n) (fun v1 v2 => forall k, AM.R K k v1 v2)) (C1.R_n m).
+
+    Definition G_n n m Γ1 Γ2 := Cross (Cross (C0.G_n n Γ1 Γ2) (fun ρ1 ρ2 => forall k, AM.G_top K k Γ1 ρ1 Γ2 ρ2)) (C1.G_n m Γ1 Γ2).
 
     Lemma V_n_wf_val_r n m v1 v2:
       V_n n m v1 v2 ->
@@ -46,13 +48,12 @@ Module M.
       unfold V_n, Cross.
       intros H.
       destruct H as [v2' [[v1' [HC0 HA]] HC1]].
-      destruct HA as [K HA].
       specialize (HA 0).
       eapply AM.V_wf_val_r in HA; eauto.
       edestruct C1.V_n_wf_val; eauto.
     Qed.
 
-    Lemma R_res_inv_l K v1 r2 :
+    Lemma R_res_inv_l v1 r2 :
       (forall i, AM.R K i (A0.Res v1) r2) ->
       exists v2, r2 = A1.Res v2 /\ (forall i, AM.V K i v1 v2).
     Proof.
@@ -72,7 +73,6 @@ Module M.
       destruct H as [r2' [[r1' [HC0 HA]] HC1]].
       apply C0.R_n_Res_inv in HC0.
       destruct HC0 as [v1' [Heqv1' HC0]]; subst.
-      destruct HA as [K HA].
       edestruct R_res_inv_l as [v2' [Heqv2' HV]]; eauto; subst.
       eexists; split; eauto.
       eapply C1.R_n_V_n; eauto.
@@ -87,14 +87,12 @@ Module M.
       destruct H as [r2' [[r1' [HC0 HA]] HC1]].
       apply C0.R_n_Res_inv in HC0.
       destruct HC0 as [v1' [Heqv1' HC0]]; subst.
-      destruct HA as [K HA].
       edestruct R_res_inv_l as [v2' [Heqv2' HV]]; eauto; subst.
 
       apply C1.R_n_Res_inv in HC1.
       2 : { specialize (HV 0).
             eapply AM.V_wf_val_r; eauto. }
       destruct HC1 as [v2'' [Heqv2'' HC1]]; subst.
-      eexists; split; eauto.
       eexists; split; eauto.
     Qed.
 
@@ -107,8 +105,7 @@ Module M.
       destruct H as [e2' [[e1' [HC0 HA]] HC1]].
       apply C0.Top_n_subset in HC0.
       apply C1.Top_n_subset in HC1.
-
-      apply (AM.trans_correct_top_subset (AM.analyze e1')) in HA.
+      apply AM.trans_correct_top_subset in HA.
       eapply Included_trans; eauto.
       eapply Included_trans; eauto.
     Qed.
@@ -120,7 +117,7 @@ Module M.
       unfold G_n, Cross.
       intros H.
       destruct H as [ρ2' [[ρ1' [HC0 HA]] HC1]].
-      specialize (HA (M.empty _) 0).
+      specialize (HA 0).
       apply AM.G_top_wf_env_r in HA.
       eapply (C1.G_n_wf_env HC1); eauto.
     Qed.
@@ -141,7 +138,7 @@ Module M.
       eexists; split; eauto.
       eexists; split; eauto.
       intros.
-      specialize (HA K k).
+      specialize (HA k).
       eapply AM.G_top_subset; eauto.
     Qed.
 
@@ -149,18 +146,19 @@ Module M.
 
   Section Adequacy.
 
-    Lemma Top_n_R_n n m e1 e2:
-      Top_n n m e1 e2 ->
+    Lemma Top_n_R_n K n m e1 e2:
+      known_map_inv K ->
+      Top_n K n m e1 e2 ->
       forall ρ1 ρ2,
         wf_env ρ2 ->
-        G_n n m (A0.occurs_free e1) (A1.occurs_free e2) ρ1 ρ2 ->
+        G_n K n m (A0.occurs_free e1) (A1.occurs_free e2) ρ1 ρ2 ->
         forall j1 r1,
           A0.bstep_fuel ρ1 e1 j1 r1 ->
           exists j2 r2,
             A1.bstep_fuel true ρ2 e2 j2 r2 /\
-            R_n n m r1 r2.
+            R_n K n m r1 r2.
     Proof.
-      intros Hrel.
+      intros HK Hrel.
       unfold Top_n, G_n, R_n, Cross in *.
       destruct Hrel as [e2' [[e1' [HC0 HA]] HC1]].
       intros.
@@ -173,12 +171,11 @@ Module M.
 
       assert (wf_env ρ2').
       {
-        specialize (HAG (M.empty _) 0).
+        specialize (HAG 0).
         eapply AM.G_top_wf_env_r; eauto.
       }
 
-      destruct (AM.analyze_sound e1') as [_ [HK _]].
-      edestruct (AM.adequacy _ _ _ HK HA) with (ρ2 := ρ2') as [j2' [r2' [Hstep2' HAR]]]; eauto.
+      edestruct (AM.adequacy K _ _ HK HA) with (ρ2 := ρ2') as [j2' [r2' [Hstep2' HAR]]]; eauto.
       - intros.
         eapply AM.G_top_subset; eauto.
         eapply C0.Top_n_subset; eauto.
@@ -190,20 +187,20 @@ Module M.
             eapply C0.Top_n_subset; eauto.
           * eapply C1.Top_n_subset; eauto.
         + eexists; eexists; split; eauto.
-          eexists; split; eauto.
     Qed.
 
     (* Termination Perservation *)
-    Theorem Top_n_preserves_termination n m e1 e2 :
-      Top_n n m e1 e2 ->
+    Theorem Top_n_preserves_termination K n m e1 e2 :
+      known_map_inv K ->
+      Top_n K n m e1 e2 ->
       forall ρ1 ρ2,
         wf_env ρ2 ->
-        G_n n m (A0.occurs_free e1) (A1.occurs_free e2) ρ1 ρ2 ->
+        G_n K n m (A0.occurs_free e1) (A1.occurs_free e2) ρ1 ρ2 ->
         forall j1 v1,
           A0.bstep_fuel ρ1 e1 j1 (A0.Res v1) ->
           exists j2 v2,
             A1.bstep_fuel true ρ2 e2 j2 (A1.Res v2) /\
-            V_n n m v1 v2.
+            V_n K n m v1 v2.
     Proof.
       intros.
       edestruct Top_n_R_n with (ρ1 := ρ1) as [j2 [r2 [Hr2 HR]]]; eauto.
@@ -217,8 +214,8 @@ Module M.
 
     Definition val_ref := Cross (Cross C0.val_ref AM.val_ref) C1.val_ref.
 
-    Lemma R_n_res_val_ref {n m v1 v2} :
-      R_n n m (A0.Res v1) (A1.Res v2) ->
+    Lemma R_n_res_val_ref {K n m v1 v2} :
+      R_n K n m (A0.Res v1) (A1.Res v2) ->
       val_ref v1 v2.
     Proof.
       unfold R_n, val_ref, Cross.
@@ -226,7 +223,6 @@ Module M.
       destruct H as [r2' [[r1' [HC0 HR]] HC1]].
       edestruct C0.R_n_Res_inv as [v1' [Heqv1' HV1]]; eauto; subst.
       eapply C0.R_n_res_val_ref in HC0; eauto.
-      destruct HR as [K HR].
       edestruct R_res_inv_l as [v2' [Heqv2' HV2]]; eauto; subst.
       eapply C1.R_n_res_val_ref in HC1; eauto.
       eexists; split; eauto.
@@ -237,11 +233,12 @@ Module M.
     Qed.
 
     (* Behavioral Refinement *)
-    Theorem Top_n_val_ref n m e1 e2 :
-      Top_n n m e1 e2 ->
+    Theorem Top_n_val_ref K n m e1 e2 :
+      known_map_inv K ->
+      Top_n K n m e1 e2 ->
       forall ρ1 ρ2,
         wf_env ρ2 ->
-        G_n n m (A0.occurs_free e1) (A1.occurs_free e2) ρ1 ρ2 ->
+        G_n K n m (A0.occurs_free e1) (A1.occurs_free e2) ρ1 ρ2 ->
         forall j1 v1,
           A0.bstep_fuel ρ1 e1 j1 (A0.Res v1) ->
           exists j2 v2,
@@ -260,31 +257,23 @@ Module M.
   Section Linking.
 
     (* Linking Preservation *)
-    Lemma Top_n_preserves_linking f w x n n' m m' e1 e2 e1' e2' :
+    Lemma Top_n_preserves_linking K f w x n n' m m' e1 e2 e1' e2' :
+      K ! f = None ->
+      K ! x = None ->
       (w \in Exposed) ->
-      Top_n n m e1 e2 ->
-      Top_n n' m' e1' e2' ->
-      Top_n (n + n') (m + m') (A0.link f x e1 e1') (A1.link f w x e2 e2').
+      Top_n K n m e1 e2 ->
+      Top_n K n' m' e1' e2' ->
+      Top_n K (n + n') (m + m') (A0.link f x e1 e1') (A1.link f w x e2 e2').
     Proof.
       unfold Top_n, Cross.
-      intro Hw.
+      intros HKf HKx Hw.
       intros.
       destruct H as [e3 [[e4 [HC0 HA1]] HC1]].
       destruct H0 as [e3' [[e4' [HC0' HA1']] HC1']].
 
       eapply (C0.Top_n_preserves_linking f x n n') in HC0; eauto.
-
-      remember (AM.analyze e4) as K1.
-      remember (AM.analyze e4') as K2.
-      remember (AM.join K1 K2) as K3.
-
-      assert (HK3A1 : AM.trans_correct_top K3 e4 e3) by admit.
-      assert (HK3A1' : AM.trans_correct_top K3 e4' e3') by admit.
-
-      eapply (AM.preserves_linking K3 f w x e4 e3 e4' e3') in HK3A1; eauto.
+      eapply (AM.preserves_linking K f w x e4 e3 e4' e3') in HA1; eauto.
       eapply (C1.Top_n_preserves_linking f w x m m') in HC1; eauto.
-      eexists; split; eauto.
-      eexists; split; eauto.
     Qed.
 
   End Linking.
